theories/Store.v
@@ -141,4 +141,29 @@ Proof.
     unfold rec_find. simpl. reflexivity.
 Qed.
 
+Example add_then_find_fileinformation : forall c,
+    let es := FileinformationStore.init c in
+    let v := {| fname := "file001"; fowner := "user"; fsize := 1024; fpermissions := 660; fmodified := "20210831T174218"; fchecksum := "42" |} in
+    let k : string := "file001" in
+    FileinformationStore.find k (FileinformationStore.add k v es) = Some v. 
+
+(* 
+Record fileinformation : Type := mkfileinformation
+     { fname : filename
+     ; fsize : N
+     ; fowner : string
+     ; fpermissions : N
+     ; fmodified : string
+     ; fchecksum : string
+     }.
+*)
+Proof.
+    intros.
+    unfold FileinformationStore.add.
+    unfold FileinformationStore.find.
+    unfold rec_find.
+    simpl. reflexivity.
+Qed.
+
+
 End Store.
